tidy up memory model
- memory model consists only of axioms
- still need to proof that axioms are consistent

partial/Memory.v
@@ -2,10 +2,6 @@
 
 Create HintDb memory.
 
-Inductive lta T n (r : T) : T -> Prop :=
-| lea_self : lta T n r (n r)
-| lea_next r' : lta T n r r' -> lta T n r (n r').
-
 
 Module Type Memory.
 
@@ -14,253 +10,72 @@ Parameter adr : Set.
 Parameter adr0 : adr.
 Parameter next : adr -> adr.
 
-Parameter dec_eq : forall (r r' : adr),  {r  = r'} + { r <> r'}.
-
-Hint Constructors lta.
-
-Infix "<" := (lta adr next) (at level 70) : memory_scope.
-
-Open Scope memory_scope.
-
-Axiom next_fresh : forall (r r' : adr), r < r' -> r <> r'.
-
 Parameter Mem : Type -> Type.
 
 
 Parameter get : forall {T}, adr -> Mem T -> option T.
 Parameter set : forall {T}, adr -> T -> Mem T -> Mem T.
 
-Axiom get_set : forall T (r : adr) (v : T) (s :  Mem T),
-    get r (set r v s) = Some v.
-Axiom get_get : forall T (r r' : adr) (v : T) (s :  Mem T),
-    r <> r' -> get r (set r' v s) = get r s.
-Axiom set_set : forall T (r : adr) (v v' : T) (s :  Mem T),
-    set r v (set r v' s) = set r v s.
-Axiom set_get : forall T (r : adr) (v : T) (s :  Mem T),
-    get r s = Some v -> set r v  s = s.
+Parameter freeFrom : forall {T}, adr -> Mem T -> Prop.
+Parameter memle : forall {T}, Mem T -> Mem T -> Prop.
 
-Notation "r ∈ s" := (exists v, get r s = Some v) (at level 70) : memory_scope.
-Notation "x ∉ y" := (~(x ∈ y)) (at level 70) : memory_scope.
 
-Parameter empty_mem : forall T, Mem T.
-
-Axiom empty_fresh : forall r {T}, r ∉ empty_mem T.
-
-Notation "s ≤ t" := (forall r, r ∈ s -> get r s = get r t) (at level 70) : memory_scope.
+Notation "s ≤ t" := (memle s t) (at level 70) : memory_scope.
+Open Scope memory_scope.
 Notation "s ≥ t" := (t ≤ s) (at level 70) : memory_scope.
 
-Notation "r <= r'" := (r < r' \/ r = r') (at level 70) : memory_scope.
+
+Axiom get_set : forall T (r : adr) (v : T) (s :  Mem T),
+    get r (set r v s) = Some v.
+
+Axiom set_set : forall T (r : adr) (v v' : T) (s :  Mem T),
+    set r v (set r v' s) = set r v s.
+
+Axiom freeFrom_set : forall {T} r (v : T) s, freeFrom r s ->  freeFrom (next r) (set r v s).
+
+
+Axiom memle_refl : forall {T} (s : Mem T), s ≤ s.
+Axiom memle_trans : forall {T} (s t u : Mem T), s ≤ t -> t ≤ u -> s ≤ u.
+
+
+Axiom memle_set : forall {T} (s : Mem T) r v, freeFrom r s -> s ≤ set r v s.
+Axiom memle_get : forall {T} (s t : Mem T) r v, s ≤ t -> get r s = v -> get r t = v.
+Axiom set_monotone : forall {T} (s t : Mem T) r v, s ≤ t -> set r v s ≤ set r v t .
+
 
 Notation "s [ r ] = v" := (get r s = Some v) (at level 70).
 Notation "s [ r := v ]" := (set r v s) (at level 70).
 
+
+Hint Resolve memle_set memle_get memle_refl set_monotone memle_trans freeFrom_set : memory.
+
 End Memory.
 
-Require Import Setoid.  
-Module MemoryTheory (Export mem : Memory).
-
-    
-
-Lemma memle_refl T (s : Mem T) : s ≤ s.
-Proof.
-  intros r D. reflexivity.
-Qed.
-
-Hint Resolve memle_refl.
-
-Lemma memle_get T r v (s t : Mem T) :
-  s ≤ t -> get r s = Some v -> get r t = Some v.
-Proof.
-  intros. assert (exists t, get r s = Some t) as E by eauto.
-  apply H in E. rewrite <- E. assumption.
-Qed.
 
 
+Module Type Empty (Import mem:Memory).
 
-Lemma memle_dom T r (s t : Mem T) : s ≤ t -> r ∈ s -> r ∈ t.
-Proof.
-  intros L D. destruct D as [v E]. eapply memle_get in E; eauto.
-Qed.
+Parameter empty_mem : forall T, Mem T.
+Axiom empty_mem_free : forall T, freeFrom adr0 (empty_mem T).
 
-Lemma memle_trans T (s t u : Mem T) : s ≤ t -> t ≤ u -> s ≤ u.
-Proof.
-  intros L1 L2 r D. rewrite L1 by assumption. eauto using memle_dom.
-Qed. 
+Hint Resolve empty_mem_free : memory.
 
-Lemma not_memle T r (s : Mem T) : r ∉ s -> get r s = None.
-Proof.
-  intros. admit. Admitted.
-(*   remember (get r s) as G. destruct G. *)
-(*   - assert (r ∈ s) as E by eauto. contradiction. *)
-(*   - reflexivity. *)
-(* Qed. *)
+End Empty.
 
-Lemma memle_set T r v (s : Mem T) : (r ∉ s) ->  s ≤ set r v s.
-Proof.
-  intros rs r' rs'.
-  remember (dec_eq r r') as R. destruct R.
-  - subst. contradiction.
-  - symmetry. apply get_get. auto.
-Qed.
+Module Type EmptyMem := Memory <+ Empty.
 
-
-
-Lemma set_dom T r r' v (s : Mem T) : r ∈ s -> r ∈ (set r' v s).
-Proof.
-  intro D. destruct (dec_eq r r').
-  - subst. eexists. rewrite get_set. eauto.
-  - destruct D. eexists. rewrite get_get by eauto. eauto.
-Qed.
-  
-Lemma set_dom_fresh T r r' v (s : Mem T) : r <> r' -> r ∈ (set r' v s) -> r ∈ s.
-Proof.
-  intros I D. destruct D. eexists. rewrite get_get in H by auto. eassumption.
-Qed.
-  
-
-
-Lemma set_monotone T r v (s t : Mem T) :
-  s ≤ t -> set r v s ≤ set r v t.
-Proof.
-  intros L r' D. destruct (dec_eq r r').
-  - subst. do 2 rewrite get_set. reflexivity.
-  - do 2 rewrite get_get by auto. apply L. eapply set_dom_fresh; eauto.
-Qed.
-
-Hint Resolve memle_set memle_get memle_refl set_monotone memle_trans : memory.
-
-
-Lemma lta_trans (r1 r2 r3 : adr) : r1 < r2 -> r2 < r3 -> r1 < r3.
-Proof.
-  intros R1 R2. induction R2;auto.
-Qed.
-
-Hint Resolve lta_trans.
-
-
-Lemma lea_lta r1 r2 r3 : r1 <= r2 -> r2 < r3 -> r1 < r3.
-Proof.
-  intros R1 R2. destruct R1. eauto. subst. assumption.
-Qed. 
-
-
-Lemma lta_lea r1 r2 r3 : r1 < r2 -> r2 <= r3 -> r1 < r3.
-Proof.
-  intros R1 R2. destruct R2. eauto. subst. assumption.
-Qed.
-
-Lemma lea_refl r : r <= r.
-Proof. auto. Qed.
-
-Lemma lta_to_lea r r' : r < r' -> r <= r'.
-Proof.
-  intro. tauto.
-Qed.
-
-Lemma lea_sym r1 r2 r3 : r1 <= r2 -> r2 <= r3 -> r1 <= r3.
-Proof.
-  intros R1 R2.
-  destruct R1;subst;try assumption.
-  destruct R2; subst;try (left; assumption).
-  left. eauto.
-Qed. 
-
-Hint Resolve lta_lea lea_lta lea_sym lea_refl.
-
-
-Definition freeFrom {T} (r : adr) (s : Mem T) := forall r', r <= r' -> r' ∉ s.
-
-Lemma freeFrom_empty r T : freeFrom r (empty_mem T).
-Proof.
-  intros r' I. apply empty_fresh.
-Qed.
-
-Hint Resolve freeFrom_empty.
-
-Lemma lta_next r r' : next r < r' -> r < r'.
-Proof.
-  intros L. remember (next r) as R. induction L;subst;auto.
-Qed.
-        
-Lemma lea_next_lta r r' : next r <= r' -> r < r'.
-Proof.
-  intros L. inversion L.
-  - apply lta_next. assumption.
-  - subst. auto.
-Qed.        
-
-Lemma lea_next r r' : next r <= r' -> r <= r'.
-Proof.
-  intros L. left. apply lea_next_lta. assumption.
-Qed.
-
-
-Lemma lea_next_neq r r' : next r <= r' -> r <> r'.
-Proof.
-  auto using next_fresh, lea_next_lta.
-Qed.
-
-Lemma freeFrom_set T r (v : T) s : freeFrom r s ->  freeFrom (next r) (set r v s).
-Proof.
-  intros F r' L.
-  assert (r <> r') as NE by auto using lea_next_neq.
-  intros I.
-  apply set_dom_fresh in I; eauto. apply F in I; auto. apply lea_next. assumption.
-Qed.
-
-
-End MemoryTheory.
 
 
 
 Module Type Truncate (Import mem:Memory).
 
 Parameter truncate : forall {T}, adr -> Mem T -> Mem T.
-Parameter dec_lta : forall (r r' : adr),  {r < r'} + { ~(r < r')}.
 
+Axiom truncate_monotone : forall {T} (s t : Mem T) r, s ≤ t -> truncate r s ≤ truncate r t.
+Axiom truncate_set : forall {T} (s : Mem T) v r , freeFrom r s -> truncate r (set r v s) = s.
 
-Axiom truncate_freeFrom : forall {T} (s : Mem T) r r', r <= r' -> r' ∉ truncate r s.
-Axiom truncate_get : forall {T} (s : Mem T) r r', ~(r <= r') -> get r' (truncate r s) = get r' s.
-Axiom funext : forall {T} (s t : Mem T), (forall r, get r s = get r t) -> s = t.
+Hint Resolve truncate_monotone truncate_set : memory.
 
 End Truncate.
 
-Module Type TruncMem := Memory <+ Truncate.
-
-Module TruncMemTheory (Export mem : TruncMem).
-Module Mem := MemoryTheory mem.
-Export Mem.
-
-Definition dec_ltea : forall (r r' : adr),  {r <= r'} + { ~r <= r'}.
-Proof.
-  intros. pose (dec_lta r r') as L. pose (dec_eq r r') as E.
-  destruct L, E; tauto.
-Qed.
-
-Lemma truncate_dom T (s : Mem T) r r' : r' ∈ truncate r s -> r' ∈ s.
-Proof.
-  intros R. pose (dec_ltea r r') as P. destruct P as [P|P].
-  - eapply truncate_freeFrom in R; auto. contradiction.
-  - destruct R. rewrite truncate_get in H by assumption. eauto.
-Qed.
-  
-Lemma truncate_monotone T (s t : Mem T) r : s ≤ t -> truncate r s ≤ truncate r t.
-Proof.
-  intros L r' E. pose (dec_ltea r r') as Q. destruct Q.
-  - eapply truncate_freeFrom in E; eauto. contradiction.
-  - do 2 erewrite truncate_get by assumption. eauto using truncate_dom.
-Qed.
-
-Lemma truncate_set T (s : Mem T) r v : freeFrom r s -> truncate r (set r v s) = s.
-Proof.
-  intro F. apply funext. intros r'. unfold freeFrom in *. pose (dec_ltea r r') as P. destruct P.
-  - pose o as o'. apply F in o'. eapply truncate_freeFrom in o.
-    do 2 rewrite not_memle by eassumption. reflexivity.
-  - rewrite truncate_get by assumption. apply get_get. intro E. subst. tauto.
-Qed.
-
-
-
-Hint Resolve truncate_monotone : memory.
-
-End TruncMemTheory.
+Module Type TruncMem := EmptyMem <+ Truncate.
